VName.thy
@@ -2,124 +2,81 @@ theory VName
 imports Main
 begin
 
-text_raw\<open>\snip{vnametype}{1}{2}{%\<close>
-datatype vname = I nat | R nat
+no_notation relcomp (infixr "O" 75)
+
+text_raw\<open>\snip{vname_otype}{1}{2}{%\<close>
+datatype vname_o = I nat | R nat | O nat
 text_raw\<open>}%endsnip\<close>
 
-instantiation vname :: linorder begin
-fun less_eq_vname :: "vname \<Rightarrow> vname \<Rightarrow> bool" where
-  "less_eq_vname (I n1) (R n2) = True" |
-  "less_eq_vname (R n1) (I n2) = False" |
-  "less_eq_vname (I n1) (I n2) = less_eq n1 n2" |
-  "less_eq_vname (R n1) (R n2) = less_eq n1 n2"
+instantiation vname_o :: linorder begin
+fun less_vname_o :: "vname_o \<Rightarrow> vname_o \<Rightarrow> bool" where
+  "less_vname_o (I n1) (I n2) = less n1 n2" |
+  "less_vname_o (I n1) (R n2) = True" |
+  "less_vname_o (I n1) (O n2) = True" |
 
-fun less_vname :: "vname \<Rightarrow> vname \<Rightarrow> bool" where
-  "less_vname (I n1) (R n2) = True" |
-  "less_vname (R n1) (I n2) = False" |
-  "less_vname (I n1) (I n2) = less n1 n2" |
-  "less_vname (R n1) (R n2) = less n1 n2"
+  "less_vname_o (R n1) (I n2) = False" |
+  "less_vname_o (R n1) (R n2) = less n1 n2" |
+  "less_vname_o (R n1) (O n2) = True" |
+
+  "less_vname_o (O n1) (I n2) = False" |
+  "less_vname_o (O n1) (R n2) = False" |
+  "less_vname_o (O n1) (O n2) = less n1 n2"
+
+fun less_eq_vname_o :: "vname_o \<Rightarrow> vname_o \<Rightarrow> bool" where
+  "less_eq_vname_o v1 v2 = (v1 < v2 \<or> v1 = v2)"
 
 instance proof
-  fix x y :: vname
+  fix x y z:: vname_o
   show "(x < y) = (x \<le> y \<and> \<not> y \<le> x)"
-  proof (induct x)
-    case (I n)
-    then show ?case
-    proof (induct y)
-      case (I m)
-      then show ?case
-        by auto
-    next
-      case (R m)
-      then show ?case
-        by simp
-    qed
-  next
-    case (R n)
-    then show ?case
-    proof (induct y)
-      case (I x)
-      then show ?case
-        by simp
-    next
-      case (R x)
-      then show ?case
-        by auto
-    qed
-  qed
-next
-  fix x :: vname
+    by (induct x y rule: less_vname_o.induct, auto)
   show "x \<le> x"
-  proof (induct x)
-    case (I x)
-    then show ?case
-      by auto
-  next
-    case (R x)
-    then show ?case
-      by auto
-  qed
-next
-  fix x y z::vname
+    by simp
   show "x \<le> y \<Longrightarrow> y \<le> z \<Longrightarrow> x \<le> z"
-  proof (induct x)
-    case (I x)
+  proof(induct x y arbitrary: z rule: less_vname_o.induct)
+    case (1 n1 n2)
     then show ?case
-    proof (induct y)
-      case (I xa)
-      then show ?case
-        apply (cases z)
-        by auto
-    next
-      case (R xa)
-      then show ?case
-        apply (cases z)
-        by auto
-    qed
+      by (cases z, auto)
   next
-    case (R x)
-    then show ?case
-    proof (induct y)
-      case (I xa)
-      then show ?case
-        apply (cases z)
-        by auto
-    next
-      case (R xa)
-      then show ?case
-        apply (cases z)
-        by auto
-    qed
+    case (2 n1 n2)
+    then show ?case 
+      by (cases z, auto)
+  next
+    case (3 n1 n2)
+    then show ?case 
+      by (cases z, auto)
+  next
+    case (4 n1 n2)
+    then show ?case 
+      by (cases z, auto)
+  next
+    case (5 n1 n2)
+    then show ?case 
+      by (cases z, auto)
+  next
+    case (6 n1 n2)
+    then show ?case 
+      by (cases z, auto)
+  next
+    case (7 n1 n2)
+    then show ?case 
+      by (cases z, auto)
+  next
+    case (8 n1 n2)
+    then show ?case 
+      by (cases z, auto)
+  next
+    case (9 n1 n2)
+    then show ?case 
+      by (cases z, auto)
   qed
-next
-  fix x y:: vname
   show "x \<le> y \<Longrightarrow> y \<le> x \<Longrightarrow> x = y"
-  proof (induct x)
-    case (I x)
-    then show ?case
-      apply (cases y)
-      by auto
-  next
-    case (R x)
-    then show ?case
-      apply (cases y)
-      by auto
-  qed
-next
-  fix x y:: vname
+    by (induct x y rule: less_vname_o.induct, auto)
   show "x \<le> y \<or> y \<le> x"
-  proof (induct x)
-    case (I x)
-    then show ?case
-      apply (cases y)
-      by auto
-  next
-    case (R x)
-    then show ?case
-      apply (cases y)
-      by auto
-  qed
+    by (induct x y rule: less_vname_o.induct, auto)
 qed
 end
+
+typedef vname = "{v :: vname_o. \<forall>n. v \<noteq> (O n)}"  morphisms vname Abs_vname
+  by auto
 
 end
